CertifyingDatalog.lean
@@ -5,3 +5,4 @@ import «CertifyingDatalog».Parsing
 import «CertifyingDatalog».TreeValidation
 import «CertifyingDatalog».Unification
 import «CertifyingDatalog».Database
+import «CertifyingDatalog».ModelChecking
